Tweaking refcell.

theories/typing/unsafe/refcell.v
@@ -26,16 +26,47 @@ Definition writing_st (q : frac) : refcell_stR := Some (Cinl (Excl ())).
 Section refcell.
   Context `{typeG Σ, refcellG Σ}.
 
-  Definition refcell_inv (l : loc) ty tid (a : lft) (γ : gname) : iProp Σ :=
+  Definition refcell_inv tid (l : loc) (γ : gname) (α : lft) ty : iProp Σ :=
     (∃ st, l ↦ #(Z_of_refcell_st st) ∗ own γ (● st) ∗
       match st return _ with
-      | None => &{a}(shift_loc l 1 ↦∗: ty.(ty_own) tid)
-      | Some (Cinr ({|agree_car := v|}, q, n)) =>
-        ∃ q', ⌜(q + q')%Qp = 1%Qp⌝ ∗ q'.[v] ∗
-              ty.(ty_shr) (a ∪ v) tid (shift_loc l 1) ∗
-              ([†v] ={lftE}=∗ &{a}(shift_loc l 1 ↦∗: ty.(ty_own) tid))
+      | None => &{α}(shift_loc l 1 ↦∗: ty.(ty_own) tid)
+      | Some (Cinr ({|agree_car := ν|}, q, n)) =>
+        ∃ q', ⌜(q + q')%Qp = 1%Qp⌝ ∗ q'.[ν] ∗
+              ty.(ty_shr) (α ∪ ν) tid (shift_loc l 1) ∗
+              ([†ν] ={lftE}=∗ &{α}(shift_loc l 1 ↦∗: ty.(ty_own) tid))
       | Some _ => True
       end)%I.
+
+  Global Instance refcell_inv_ne n tid l γ α :
+    Proper (dist n ==> dist n) (refcell_inv tid l γ α).
+  Proof.
+    intros ty1 ty2 Hty. unfold refcell_inv.
+    repeat (f_contractive || f_equiv || apply Hty).
+  Qed.
+
+  Lemma refcell_inv_proper E L tid l γ α1 α2 ty1 ty2 :
+    lctx_lft_incl E L α2 α1 → eqtype E L ty1 ty2 →
+    lft_ctx -∗ elctx_interp_0 E -∗ ⌜llctx_interp_0 L⌝ -∗
+    refcell_inv tid l γ α1 ty1 -∗ refcell_inv tid l γ α2 ty2.
+  Proof.
+    (* TODO : this proof is essentially [solve_proper], but within the logic.
+              It would easily gain from some automation. *)
+    iIntros (Hα Hty%eqtype_unfold) "#LFT #HE #HL H". unfold refcell_inv.
+    iDestruct (Hty with "LFT HE HL") as "(% & Hown & Hshr)".
+    iAssert (□ (&{α1} shift_loc l 1 ↦∗: ty_own ty1 tid -∗
+                &{α2} shift_loc l 1 ↦∗: ty_own ty2 tid))%I with "[]" as "#Hb".
+    { iIntros "!# H". iApply (bor_shorten with "[]"). by iApply Hα.
+      iApply bor_iff_proper; last done.
+      iSplit; iIntros "!>!#H"; iDestruct "H" as (vl) "[Hf H]"; iExists vl;
+      iFrame; by iApply "Hown". }
+    iDestruct "H" as (st) "H"; iExists st;
+      iDestruct "H" as "($&$&H)"; destruct st as [[|[[[]]]|]|]; try done;
+      last by iApply "Hb".
+    iDestruct "H" as (q') "(Heq & Htok & Hs & H†)". iExists q'. iFrame. iSplitL "Hs".
+    - iApply (ty_shr_mono); first done; last by iApply "Hshr".
+      by iApply lft_glb_mono; [iApply Hα|iApply lft_incl_refl].
+    - iIntros "?". iApply ("Hb" with ">"). by iApply "H†".
+  Qed.
 
   Program Definition refcell (ty : type) :=
     {| ty_size := S ty.(ty_size);
@@ -45,7 +76,7 @@ Section refcell.
          | _ => False
          end%I;
        ty_shr κ tid l :=
-         (∃ a γ, κ ⊑ a ∗ &na{a, tid, lrustN}(refcell_inv l ty tid a γ))%I |}.
+         (∃ α γ, κ ⊑ α ∗ &na{α, tid, lrustN}(refcell_inv tid l γ α ty))%I |}.
   Next Obligation.
     iIntros (??[|[[]|]]); try iIntros "[]". rewrite ty_size_eq.
     iIntros "[_ %]!%/=". congruence.
@@ -64,7 +95,7 @@ Section refcell.
       iExists (#n'::vl'). rewrite heap_mapsto_vec_cons. iFrame "∗%". }
     iMod (bor_sep with "LFT H") as "[Hn Hvl]". done.
     iMod (bor_acc_cons with "LFT Hn Htok") as "[H Hclose]". done.
-    iAssert ((q / 2).[κ] ∗ ▷ ∃ γ, refcell_inv l ty tid κ γ)%I with ">[-Hclose]"
+    iAssert ((q / 2).[κ] ∗ ▷ ∃ γ, refcell_inv tid l γ κ ty)%I with ">[-Hclose]"
       as "[$ HQ]"; last first.
     { iMod ("Hclose" with "* HQ []") as "[Hb $]".
       - iIntros "!> H !>". iNext. iDestruct "H" as (γ st) "(? & _ & _)".
@@ -73,16 +104,16 @@ Section refcell.
         iExists κ, γ. iSplitR. by iApply lft_incl_refl. by iApply bor_na. }
     clear dependent n. iDestruct "H" as ([|n|[]]) "[Hn >%]"; try lia.
     - iFrame. iMod (own_alloc (● None)) as (γ) "Hst". done. iExists γ, None. by iFrame.
-    - iMod (lft_create with "LFT") as (v) "[[Htok1 Htok2] _]". done.
+    - iMod (lft_create with "LFT") as (ν) "[[Htok1 Htok2] _]". done.
       iMod (own_alloc
-         (● Some (Cinr (to_agree (v : leibnizC _), (1/2)%Qp, n)))) as (γ) "Hst".
+         (● Some (Cinr (to_agree (ν : leibnizC _), (1/2)%Qp, n)))) as (γ) "Hst".
       { by apply auth_auth_valid. }
       destruct (Qp_lower_bound (1/2) (q/2)) as (q' & q1 & q2 & H12 & ->). rewrite H12.
       iDestruct "Htok'" as "[Htok' $]". iDestruct "Htok1" as "[Htok1 Htok1']".
       iApply (fupd_mask_mono lftE). done.
-      iMod (rebor _ _ (κ∪v) with "LFT [] Hvl") as "[Hvl Hh]". done.
+      iMod (rebor _ _ (κ ∪ ν) with "LFT [] Hvl") as "[Hvl Hh]". done.
       { iApply lft_le_incl. apply gmultiset_union_subseteq_l. }
-      iMod (ty_share _ _ (κ∪v) _ _ q' with "LFT Hvl [Htok' Htok1]")
+      iMod (ty_share _ _ (κ ∪ ν) _ _ q' with "LFT Hvl [Htok' Htok1]")
         as "[Hshr Htok]". done.
       { rewrite -lft_tok_sep. iFrame. }
       rewrite -lft_tok_sep. iDestruct "Htok" as "[$ Htok]".
@@ -94,40 +125,30 @@ Section refcell.
       iFrame. iExists _, _. by iFrame.
   Qed.
   Next Obligation.
-    iIntros (?????) "LFT #Hκ H". iDestruct "H" as (a γ) "[#??]".
+    iIntros (?????) "LFT #Hκ H". iDestruct "H" as (α γ) "[#??]".
     iExists _, _. iFrame. iApply lft_incl_trans; auto.
   Qed.
 
   Global Instance refcell_ne n : Proper (dist n ==> dist n) refcell.
   Proof.
-    move=>??[[]]/=Hsz Hown Hshr. split; [split|]; simpl. congruence.
-    - f_contractive=>tid vl. repeat f_equiv. apply Hown.
-    - intros κ tid l. unfold refcell_inv.
-      repeat (f_contractive || f_equiv); apply dist_S.
-      apply Hshr. apply Hown. apply Hown.
+    move=>ty1 ty2 Hty. split; [split|]; simpl.
+    - f_equiv. apply Hty.
+    - f_contractive=>tid vl. repeat f_equiv. apply Hty.
+    - intros κ tid l. by repeat f_equiv.
   Qed.
 
   Global Instance refcell_mono E L : Proper (eqtype E L ==> subtype E L) refcell.
   Proof.
     (* TODO : this proof is essentially [solve_proper], but within the logic.
               It would easily gain from some automation. *)
-    iIntros (ty1 ty2 EQ%eqtype_unfold) "#LFT #HE #HL".
-    iDestruct (EQ with "LFT HE HL") as "(% & #Hown & #Hshr)".
+    iIntros (ty1 ty2 EQ) "#LFT #HE #HL". pose proof EQ as EQ'%eqtype_unfold.
+    iDestruct (EQ' with "LFT HE HL") as "(% & #Hown & #Hshr)".
     iSplit; [|iSplit; iIntros "!# * H"].
     - iPureIntro. simpl. congruence.
     - destruct vl as [|[[]|]]; try done. iDestruct "H" as "[$ H]". by iApply "Hown".
     - iDestruct "H" as (a γ) "[Ha H]". iExists a, γ. iFrame.
-      iApply (na_bor_iff_proper with "[] H"). iNext. iAlways.
-      iAssert (□ (&{a} shift_loc l 1 ↦∗: ty_own ty1 tid ↔
-                  &{a} shift_loc l 1 ↦∗: ty_own ty2 tid))%I as "#Hbiff".
-      { iSplit; iIntros "!#H"; iApply (bor_iff_proper with "[] H"); iIntros "!>!#"; 
-        iSplit; iIntros "H"; iDestruct "H" as (vl) "[Hf H]"; iExists vl; iFrame;
-          by iApply "Hown". }
-      iSplit; iIntros "H"; iDestruct "H" as (st) "H"; iExists st;
-        iDestruct "H" as "($&$&H)"; destruct st as [[|[[[]]]|]|]; try done;
-        (try by iApply "Hbiff");
-      iDestruct "H" as (q') "(Heq & Htok & Hs & H†)"; iExists q'; iFrame;
-      (iSplitL "Hs"; [by iApply "Hshr"| iIntros "?"; iApply "Hbiff"; by iApply "H†"]).
+      iApply na_bor_iff_proper; last done.
+      iSplit; iIntros "!>!# H"; by iApply refcell_inv_proper.
   Qed.
   Lemma refcell_mono' E L ty1 ty2 :
     eqtype E L ty1 ty2 → subtype E L (refcell ty1) (refcell ty2).
